adapted to Isabelle b0b9a10e4bf4

Analysis/Normal_Distribution.thy
@@ -3,121 +3,195 @@
    Author: Johannes Hölzl *)
 
 theory Normal_Distribution
-  imports Convolution
+  imports Probability
 begin
+
+lemma filterlim_power2_at_top[intro]: "filterlim (\<lambda>(x::real). x\<^sup>2) at_top at_top"
+  by (auto intro!: filterlim_at_top_mult_at_top filterlim_ident simp: power2_eq_square)
+
+lemma distributed_integrable_var:
+  fixes X :: "'a \<Rightarrow> real"
+  shows "distributed M lborel X (\<lambda>x. ereal (f x)) \<Longrightarrow> integrable lborel (\<lambda>x. f x * x) \<Longrightarrow> integrable M X"
+  using distributed_integrable[of M lborel X f "\<lambda>x. x"] by simp
+
+lemma (in ordered_comm_monoid_add) setsum_pos: 
+  "finite I \<Longrightarrow> I \<noteq> {} \<Longrightarrow> (\<And>i. i \<in> I \<Longrightarrow> 0 < f i) \<Longrightarrow> 0 < setsum f I"
+  by (induct I rule: finite_ne_induct) (auto intro: add_pos_pos)
+
+lemma ln_sqrt: "0 < x \<Longrightarrow> ln (sqrt x) = ln x / 2"
+  by (simp add: ln_powr powr_numeral ln_powr[symmetric] mult_commute)
+
+lemma distr_cong: "M = K \<Longrightarrow> sets N = sets L \<Longrightarrow> (\<And>x. x \<in> space M \<Longrightarrow> f x = g x) \<Longrightarrow> distr M N f = distr K L g"
+  using sets_eq_imp_space_eq[of N L] by (simp add: distr_def Int_def cong: rev_conj_cong)
+
+lemma AE_borel_affine: 
+  fixes P :: "real \<Rightarrow> bool"
+  shows "c \<noteq> 0 \<Longrightarrow> Measurable.pred borel P \<Longrightarrow> AE x in lborel. P x \<Longrightarrow> AE x in lborel. P (t + c * x)"
+  by (subst lborel_real_affine[where t="- t / c" and c="1 / c"])
+     (simp_all add: AE_density AE_distr_iff field_simps)
+
+lemma density_distr:
+  assumes [measurable]: "f \<in> borel_measurable N" "X \<in> measurable M N"
+  shows "density (distr M N X) f = distr (density M (\<lambda>x. f (X x))) N X"
+  by (intro measure_eqI)
+     (auto simp add: emeasure_density nn_integral_distr emeasure_distr
+           split: split_indicator intro!: nn_integral_cong)
+
+lemma ereal_mult_indicator: "ereal (x * indicator A y) = ereal x * indicator A y"
+  by (simp split: split_indicator)
+
+lemma (in prob_space) distributed_affine:
+  fixes f :: "real \<Rightarrow> ereal"
+  assumes f: "distributed M lborel X f"
+  assumes c: "c \<noteq> 0"
+  shows "distributed M lborel (\<lambda>x. t + c * X x) (\<lambda>x. f ((x - t) / c) / \<bar>c\<bar>)"
+  unfolding distributed_def
+proof safe
+  have [measurable]: "f \<in> borel_measurable borel"
+    using f by (simp add: distributed_def)
+  have [measurable]: "X \<in> borel_measurable M"
+    using f by (simp add: distributed_def)
+
+  show "(\<lambda>x. f ((x - t) / c) / \<bar>c\<bar>) \<in> borel_measurable lborel"
+    by simp
+  show "random_variable lborel (\<lambda>x. t + c * X x)"
+    by simp
+  
+  have "AE x in lborel. 0 \<le> f x"
+    using f by (simp add: distributed_def)
+  from AE_borel_affine[OF _ _ this, where c="1/c" and t="- t / c"] c
+  show "AE x in lborel. 0 \<le> f ((x - t) / c) / ereal \<bar>c\<bar>"
+    by (auto simp add: field_simps)
+
+  have eq: "\<And>x. ereal \<bar>c\<bar> * (f x / ereal \<bar>c\<bar>) = f x"
+    using c by (simp add: divide_ereal_def mult_ac one_ereal_def[symmetric])
+    
+  have "density lborel f = distr M lborel X"
+    using f by (simp add: distributed_def)
+  with c show "distr M lborel (\<lambda>x. t + c * X x) = density lborel (\<lambda>x. f ((x - t) / c) / ereal \<bar>c\<bar>)"
+    by (subst (2) lborel_real_affine[where c="c" and t="t"])
+       (simp_all add: density_density_eq density_distr distr_distr field_simps eq cong: distr_cong)
+qed
+
+lemma (in prob_space) distributed_affineI:
+  fixes f :: "real \<Rightarrow> ereal"
+  assumes f: "distributed M lborel (\<lambda>x. (X x - t) / c) (\<lambda>x. \<bar>c\<bar> * f (x * c + t))"
+  assumes c: "c \<noteq> 0"
+  shows "distributed M lborel X f"
+proof -
+  have eq: "\<And>x. f x * ereal \<bar>c\<bar> / ereal \<bar>c\<bar> = f x"
+    using c by (simp add: divide_ereal_def mult_ac one_ereal_def[symmetric])
+
+  show ?thesis
+    using distributed_affine[OF f c, where t=t] c
+    by (simp add: field_simps eq)
+qed
 
 definition normal_density :: "real \<Rightarrow> real \<Rightarrow> real \<Rightarrow> real" where
   "normal_density \<mu> \<sigma> x = 1 / sqrt (2 * pi * \<sigma>\<^sup>2) * exp (-(x - \<mu>)\<^sup>2/ (2 * \<sigma>\<^sup>2))"
 
-abbreviation "standard_normal_density == normal_density 0 1"
+abbreviation standard_normal_density :: "real \<Rightarrow> real" where
+  "standard_normal_density \<equiv> normal_density 0 1"
 
-lemma standard_normal_density_def: "standard_normal_density x = (1 / sqrt (2 * pi)) * exp (- x\<^sup>2 /2)"
+lemma standard_normal_density_def: "standard_normal_density x = (1 / sqrt (2 * pi)) * exp (- x\<^sup>2 / 2)"
   unfolding normal_density_def by simp
 
 lemma borel_measurable_normal_density[measurable]: "normal_density \<mu> \<sigma> \<in> borel_measurable borel"
   by (auto simp: normal_density_def[abs_def])
 
-lemma aux3:
-  fixes s::real
-  shows "(\<integral>\<^sup>+ x. ereal (x * exp (- x\<^sup>2 * (1 + s\<^sup>2))) * indicator {0..} x \<partial>lborel) =  1 / (2 * (1 + s\<^sup>2))"
-proof -  
-  have "(\<integral>\<^sup>+ x. ereal (x * exp (- x\<^sup>2 * (1 + s\<^sup>2))) * indicator {0..} x \<partial>lborel) = ereal (0 - (\<lambda>x. ((-1 / (2 * (1 + s\<^sup>2)))) * exp (-x\<^sup>2 * (1 + s\<^sup>2))) 0)"
-    proof(rule nn_integral_FTC_atLeast, auto intro!: derivative_eq_intros 
-        simp: mult_nonneg_nonneg field_simps add_nonneg_eq_0_iff)
+lemma nn_integral_even_function:
+  fixes f :: "real \<Rightarrow> ereal"
+  assumes [measurable]: "f \<in> borel_measurable borel"
+  assumes even: "\<And>x. f x = f (- x)"
+  shows "(\<integral>\<^sup>+x. f x \<partial>lborel) = 2 * (\<integral>\<^sup>+x. f x * indicator {0 ..} x \<partial>lborel)"
+proof -
+  def f' \<equiv> "\<lambda>x. max 0 (f x)"
+  have [measurable]: "f' \<in> borel_measurable borel"
+    by (simp add: f'_def)
+  
+  { fix x :: ereal have "2 * x = x + x"
+      by (cases x) auto }
+  note two_mult = this
+
+  have "(\<integral>\<^sup>+x. f x \<partial>lborel) = (\<integral>\<^sup>+x. f' x \<partial>lborel)"
+    unfolding f'_def nn_integral_max_0 ..
+  also have "\<dots> = (\<integral>\<^sup>+x. f' x * indicator {0 ..} x + f' x * indicator {.. 0} x \<partial>lborel)"
+    by (intro nn_integral_cong_AE AE_I[where N="{0}"]) (auto split: split_indicator_asm)
+  also have "\<dots> = (\<integral>\<^sup>+x. f' x * indicator {0 ..} x \<partial>lborel) + (\<integral>\<^sup>+x. f' x * indicator {.. 0} x \<partial>lborel)"
+    by (intro nn_integral_add) (auto simp: f'_def)
+  also have "(\<integral>\<^sup>+x. f' x * indicator {.. 0} x \<partial>lborel) = (\<integral>\<^sup>+x. f' x * indicator {0 ..} x \<partial>lborel)"
+    using even
+    by (subst nn_integral_real_affine[where c="-1" and t=0])
+       (auto simp: f'_def one_ereal_def[symmetric] split: split_indicator intro!: nn_integral_cong)
+  also have "(\<integral>\<^sup>+x. f' x * indicator {0 ..} x \<partial>lborel) = (\<integral>\<^sup>+x. f x * indicator {0 ..} x \<partial>lborel)"
+    unfolding f'_def by (subst (2) nn_integral_max_0[symmetric]) (auto intro!: nn_integral_cong split: split_indicator split_max)
+  finally show ?thesis
+    unfolding two_mult by simp
+qed
+
+lemma nn_integral_gaussian: "(\<integral>\<^sup>+x. (exp (- x\<^sup>2)) \<partial>lborel) = sqrt pi"
+proof -
+  let ?pI = "\<lambda>f. (\<integral>\<^sup>+s. f (s::real) * indicator {0..} s \<partial>lborel)"
+  let ?gauss = "\<lambda>x. exp (- x\<^sup>2)"
+
+  have "?pI ?gauss * ?pI ?gauss = ?pI (\<lambda>s. ?pI (\<lambda>x. ereal (x * exp (-x\<^sup>2 * (1 + s\<^sup>2)))))"
+  proof-
+    let ?ff= "\<lambda>(x, s). ((x * exp (- x\<^sup>2 * (1 + s\<^sup>2)) * indicator {0<..} s * indicator {0<..} x)) :: real"
+  
+    have *: "?pI ?gauss = (\<integral>\<^sup>+x. ?gauss x * indicator {0<..} x \<partial>lborel)"
+      by (intro nn_integral_cong_AE AE_I[where N="{0}"]) (auto split: split_indicator)
+  
+    have "?pI ?gauss * ?pI ?gauss = (\<integral>\<^sup>+x. \<integral>\<^sup>+s. ?ff (x, s) \<partial>lborel \<partial>lborel)"
+      unfolding *
+      apply (auto simp: nn_integral_nonneg nn_integral_cmult[symmetric])
+      apply (auto intro!: nn_integral_cong split:split_indicator)
+      apply (auto simp: nn_integral_multc[symmetric])
+      apply (subst nn_integral_real_affine[where t="0" and c="x"])
+      by (auto simp: mult_exp_exp nn_integral_cmult[symmetric] field_simps zero_less_mult_iff
+          intro!: nn_integral_cong split:split_indicator)
+    also have "... = \<integral>\<^sup>+ (s::real). \<integral>\<^sup>+ (x::real). ?ff (x, s) \<partial>lborel \<partial>lborel"
+      by (rule lborel_pair.Fubini[symmetric]) auto
+    also have "... = ?pI (\<lambda>s. ?pI (\<lambda>x. ereal (x * exp (-x\<^sup>2 * (1 + s\<^sup>2)))))"
+      by (rule nn_integral_cong_AE) (auto intro!: nn_integral_cong_AE AE_I[where N="{0}"] split: split_indicator_asm)
+    finally show ?thesis
+      by simp
+  qed
+  also have "\<dots> = ?pI (\<lambda>s. ereal (1 / (2 * (1 + s\<^sup>2))))"
+  proof (intro nn_integral_cong ereal_right_mult_cong)
+    fix s :: real show "?pI (\<lambda>x. ereal (x * exp (-x\<^sup>2 * (1 + s\<^sup>2)))) = ereal (1 / (2 * (1 + s\<^sup>2)))"
+    proof (subst nn_integral_FTC_atLeast)
       have "((\<lambda>a. - (exp (- (a\<^sup>2 * (1 + s\<^sup>2))) / (2 + 2 * s\<^sup>2))) ---> (- (0 / (2 + 2 * s\<^sup>2)))) at_top"
         apply (intro tendsto_intros filterlim_compose[OF exp_at_bot] filterlim_compose[OF filterlim_uminus_at_bot_at_top])
         apply (subst mult_commute)         
         by (auto intro!: filterlim_tendsto_pos_mult_at_top filterlim_at_top_mult_at_top[OF filterlim_ident filterlim_ident] 
           simp: add_pos_nonneg  power2_eq_square add_nonneg_eq_0_iff)
-      then show "((\<lambda>a. - (exp (- a\<^sup>2 - a\<^sup>2 * s\<^sup>2) / (2 + 2 * s\<^sup>2))) ---> 0) at_top" by (simp add: field_simps)
-   qed 
-  then show ?thesis by simp
-qed
-
-lemma aux4:
-    "(\<integral>\<^sup>+ x. ereal (exp (- x\<^sup>2) * indicator {0..} x) \<partial>lborel) * (\<integral>\<^sup>+ x. ereal (exp (- x\<^sup>2) * indicator {0..} x) \<partial>lborel) =
-    \<integral>\<^sup>+ s. (\<integral>\<^sup>+ x. ereal (x * exp (- x\<^sup>2 * (1 + s\<^sup>2)) * indicator {0..} x) \<partial>lborel) * indicator {0..} s \<partial>lborel"
-proof-
-  let ?f = "\<lambda>x. exp (- x\<^sup>2) * indicator {0..} x"
-  let ?ff= "\<lambda>(x::real, s::real). ((x * exp (- x\<^sup>2 * (1 + s\<^sup>2)) * indicator {0<..} s * indicator {0<..} x))"
-
-  have *: "(integral\<^sup>N lborel ?f) = (integral\<^sup>N lborel  (\<lambda>x. exp (- x\<^sup>2) * indicator {0<..} x))"
-    by (auto intro!: nn_integral_cong_AE split:split_indicator)
-       (rule AE_I[where N="{0}"], auto)
-
-  have "(integral\<^sup>N lborel ?f) *  (integral\<^sup>N lborel ?f) = (integral\<^sup>N lborel (\<lambda>(x::real). (integral\<^sup>N lborel (\<lambda>(s::real). x * exp (-x\<^sup>2 * (1 + s\<^sup>2)) * indicator {0<..} s * indicator {0<..} x))))"
-    apply (simp add: *)
-    apply (auto simp: nn_integral_nonneg nn_integral_cmult[symmetric])
-    apply (auto intro!: nn_integral_cong split:split_indicator)
-    apply (auto simp: nn_integral_multc[symmetric])
-    apply (subst nn_integral_real_affine[where t="0" and c="x"])
-    by (auto simp: mult_nonneg_nonneg mult_pos_pos mult_exp_exp nn_integral_cmult[symmetric] field_simps power_mult_distrib zero_less_mult_iff
-        intro!: nn_integral_cong split:split_indicator)
-
-  also have "... = \<integral>\<^sup>+ (x::real). \<integral>\<^sup>+ (s::real). ?ff (x, s) \<partial>lborel \<partial>lborel" by (auto intro!: nn_integral_cong)
-  also have "... = \<integral>\<^sup>+ (s::real). \<integral>\<^sup>+ (x::real). ?ff (x, s) \<partial>lborel \<partial>lborel" by (rule lborel_pair.Fubini[symmetric]) auto
-  also have "... = (integral\<^sup>N lborel (\<lambda>(s::real). (integral\<^sup>N lborel (\<lambda>(x::real). x * exp (-x\<^sup>2 * (1 + s\<^sup>2)) * indicator {0..} x) * indicator {0..} s)))"
-    apply (rule nn_integral_cong_AE)
-    by (auto intro!: nn_integral_cong_AE AE_I[where N="{0}"] split: split_indicator)
-   finally show ?thesis by fast
-qed
-
-lemma gaussian_integral_positive: "(\<integral>\<^sup>+x. (exp (- x\<^sup>2)) \<partial>lborel) = sqrt pi"
-proof -
-(*  let ?i = "\<lambda>f. (\<integral>\<^sup>+ x. ereal (f x) * indicator {0..} x \<partial>lborel)" *)
-  let ?I = "\<integral>\<^sup>+x. (exp (- x\<^sup>2)) \<partial>lborel"   
-  let ?f = "\<lambda>x. exp (- x\<^sup>2) * indicator {0..} x"
-  let ?ff = "\<lambda>(x::real, s::real). ((x * exp (- x\<^sup>2 * (1 + s\<^sup>2)) * indicator {0..} s * indicator {0..} x))"
-  
-  have 1: "?I\<^sup>2 = 4 * (integral\<^sup>N lborel ?f) * (integral\<^sup>N lborel ?f)"
-    apply (cases "integral\<^sup>N lborel ?f")
-    by (auto simp: power2_eq_square ac_simps nn_integral_even_function)
-
-  have 2: "(integral\<^sup>N lborel ?f) * (integral\<^sup>N lborel ?f) = \<integral>\<^sup>+ s. (\<integral>\<^sup>+ x. ereal (x * exp (- x\<^sup>2 * (1 + s\<^sup>2)) * indicator {0..} x) \<partial>lborel) * indicator {0..} s \<partial>lborel"
-    by(rule aux4)
-
-  fix s::real
-    
-  let ?I1 =" \<integral>\<^sup>+ x. ereal (x * exp (- x\<^sup>2 * (1 + s\<^sup>2))) * indicator {0..} x \<partial>lborel"
-  have 3:"?I1 = 1 / (2 * (1 + s\<^sup>2)) "
-    by(rule aux3)
-
-  have "(\<integral>\<^sup>+ x. ereal (x * exp (- x\<^sup>2 * (1 + s\<^sup>2)) * indicator {0..} s * indicator {0..} x) \<partial>lborel) = 
-        \<integral>\<^sup>+ x. indicator {0..} s * ereal (x * exp (- x\<^sup>2 * (1 + s\<^sup>2)) ) * indicator {0..} x \<partial>lborel"
-    by(auto intro!: nn_integral_cong split:split_indicator)
-
-  then have [simp]:"... =  (indicator {0..} s) *  1 / (2 * (1 + s\<^sup>2))" using 3 by (auto split:split_indicator)
-     
-  have 6:"integral\<^sup>N lborel (\<lambda>(s::real). (integral\<^sup>N lborel (\<lambda>(x::real). x * exp (-x\<^sup>2 * (1 + s\<^sup>2)) * indicator {0..} x) * indicator {0..} s)) 
-         = integral\<^sup>N lborel (\<lambda>(s::real). ereal (1 / (2 * (1 + s\<^sup>2))) * (indicator {0..} s))"
-    by (subst aux3[symmetric]) (auto simp: aux3[symmetric] intro!: nn_integral_cong split: split_indicator)
-        
-  also have "... = ereal ( pi / 4 - (\<lambda>x. arctan x / 2) 0)"
-    apply (rule nn_integral_FTC_atLeast, auto)
-    apply (intro derivative_eq_intros, auto simp:inverse_eq_divide distrib_left) 
-    apply (simp add:field_simps add_nonneg_eq_0_iff)
-    proof-
-      have "((\<lambda>a. arctan a / 2) ---> (pi / 2) / 2 ) at_top"
-      apply (intro tendsto_intros)
-      by (simp_all add: tendsto_arctan_at_top)
-      then show "((\<lambda>a. arctan a / 2) ---> pi / 4) at_top" by simp
-   qed
-  also have "... = pi / 4" by simp
-  finally have "(integral\<^sup>N lborel (\<lambda>(s::real). (integral\<^sup>N lborel (\<lambda>(x::real). x * exp (-x\<^sup>2 * (1 + s\<^sup>2)) * indicator {0..} x) * indicator {0..} s))) = pi / 4"
-    by linarith
-
-  with 1 2 3 have 8:" (\<integral>\<^sup>+ x. ereal (exp (- x\<^sup>2)) \<partial>lborel)\<^sup>2 = pi" by(simp add:field_simps)
-  
+      then show "((\<lambda>a. - (exp (- a\<^sup>2 - s\<^sup>2 * a\<^sup>2) / (2 + 2 * s\<^sup>2))) ---> 0) at_top"
+        by (simp add: field_simps)
+    qed (auto intro!: derivative_eq_intros simp: field_simps add_nonneg_eq_0_iff)
+  qed
+  also have "... = ereal (pi / 4)"
+  proof (subst nn_integral_FTC_atLeast)
+    show "((\<lambda>a. arctan a / 2) ---> (pi / 2) / 2 ) at_top"
+      by (intro tendsto_intros) (simp_all add: tendsto_arctan_at_top)
+  qed (auto intro!: derivative_eq_intros simp: add_nonneg_eq_0_iff field_simps power2_eq_square)
+  finally have "?pI ?gauss^2 = pi / 4"
+    by (simp add: power2_eq_square)
+  then have "?pI ?gauss = sqrt (pi / 4)"
+    using power_eq_iff_eq_base[of 2 "real (?pI ?gauss)" "sqrt (pi / 4)"]
+      nn_integral_nonneg[of lborel "\<lambda>x. ?gauss x * indicator {0..} x"]
+    by (cases "?pI ?gauss") auto
   then show ?thesis
-    apply (cases "(\<integral>\<^sup>+ x. ereal (exp (- x\<^sup>2)) \<partial>lborel)", auto intro!: power2_eq_imp_eq[where y= "sqrt pi"])
-    by (metis ereal_less_eq(5) nn_integral_nonneg)    
+    by (subst nn_integral_even_function) (auto simp add: real_sqrt_divide)
 qed
 
-lemma gaussian_integral: "(\<integral>x. (exp (- x\<^sup>2)) \<partial>lborel) = (sqrt pi)"
-  by (auto intro!: lebesgue_integral_eq_nn_integral gaussian_integral_positive)
+lemma has_bochner_integral_gaussian: "has_bochner_integral lborel (\<lambda>x. exp (- x\<^sup>2)) (sqrt pi)"
+  by (auto intro!: nn_integral_gaussian has_bochner_integral_nn_integral)
 
-lemma gaussian_integrable[intro]: "integrable lborel (\<lambda>x. exp (- x\<^sup>2)::real)"
-  by (auto intro!: integrable_if_nn_integral gaussian_integral_positive)
+lemma integral_gaussian: "(\<integral>x. (exp (- x\<^sup>2)) \<partial>lborel) = sqrt pi"
+  using has_bochner_integral_gaussian by (rule has_bochner_integral_integral_eq)
+
+lemma integrable_gaussian[intro]: "integrable lborel (\<lambda>x. exp (- x\<^sup>2)::real)"
+  using has_bochner_integral_gaussian by rule
 
 context
   fixes \<sigma> :: real
@@ -127,38 +201,24 @@ begin
 lemma nn_integral_normal_density: "(\<integral>\<^sup>+x. normal_density \<mu> \<sigma> x \<partial>lborel) = 1"
   unfolding normal_density_def
   apply (subst times_ereal.simps(1)[symmetric],subst nn_integral_cmult)
-  apply (auto simp: mult_nonneg_nonneg)
+  apply auto
   apply (subst nn_integral_real_affine[where t=\<mu> and  c="(sqrt 2) * \<sigma>"])
-  by (auto simp: power_mult_distrib gaussian_integral_positive mult_nonneg_nonneg 
-    real_sqrt_mult one_ereal_def divide_minus_left)
+  by (auto simp: power_mult_distrib nn_integral_gaussian real_sqrt_mult one_ereal_def)
 
 lemma 
   shows normal_positive: "\<And>x. 0 < normal_density \<mu> \<sigma> x"
-  and normal_non_negative: "\<And>x. 0 \<le> normal_density \<mu> \<sigma> x" 
-  unfolding normal_density_def
-  by (auto simp: mult_nonneg_nonneg divide_nonneg_nonneg mult_pos_pos divide_pos_pos)
-
+  and normal_nonneg: "\<And>x. 0 \<le> normal_density \<mu> \<sigma> x" 
+  by (auto simp: normal_density_def)
 
 lemma integrable_normal[intro]: "integrable lborel (normal_density \<mu> \<sigma>)"
-   by (auto intro!: integrable_if_nn_integral[where x=1] normal_non_negative 
-            simp: nn_integral_normal_density one_ereal_def)
+  by (auto intro!: integrableI_nn_integral_finite simp: nn_integral_normal_density normal_nonneg)
 
 lemma integral_normal_density[simp]: "(\<integral>x. normal_density \<mu> \<sigma> x \<partial>lborel) = 1"
-  using nn_integral_normal_density
-  by (subst lebesgue_integral_eq_nn_integral)
-     (auto intro!: normal_non_negative simp: one_ereal_def)
+  by (simp add: integral_eq_nn_integral normal_nonneg nn_integral_normal_density)
 
 lemma prob_space_normal_density:
   "prob_space (density lborel (normal_density \<mu> \<sigma>))" (is "prob_space ?D")
-proof-
-  have "emeasure ?D (space ?D) =  emeasure (density lborel (\<lambda>x. normal_density \<mu> \<sigma> x)) UNIV"
-    unfolding normal_density_def by auto
-  also have "... = \<integral>\<^sup>+ x.  normal_density \<mu> \<sigma> x \<partial>lborel"
-    by (subst emeasure_density[of "\<lambda>x. normal_density \<mu> \<sigma> x" lborel UNIV]) auto
-  also have " ...  = 1"
-    by (rule nn_integral_normal_density)
-  finally show "prob_space ?D" by rule
-qed
+  proof qed (simp add: emeasure_density nn_integral_normal_density)
 
 end
 
@@ -169,7 +229,7 @@ lemma (in prob_space) normal_density_affine:
 proof -
   have eq: "\<And>x. \<bar>\<alpha>\<bar> * normal_density (\<beta> + \<alpha> * \<mu>) (\<bar>\<alpha>\<bar> * \<sigma>) (x * \<alpha> + \<beta>) =
     normal_density \<mu> \<sigma> x"
-    by (simp add: normal_density_def real_sqrt_mult power_mult_distrib field_simps)
+    by (simp add: normal_density_def real_sqrt_mult field_simps)
        (simp add: power2_eq_square field_simps)
   show ?thesis
     by (rule distributed_affineI[OF _ `\<alpha> \<noteq> 0`, where t=\<beta>]) (simp_all add: eq X)
@@ -177,14 +237,14 @@ qed
 
 lemma (in prob_space) normal_standard_normal_convert:
   assumes pos_var[simp, arith]: "0 < \<sigma>"
-  shows "distributed M lborel X (normal_density  \<mu> \<sigma>) = distributed M lborel (\<lambda>x. (X x - \<mu>)/ \<sigma>) standard_normal_density"
-proof(auto)
+  shows "distributed M lborel X (normal_density  \<mu> \<sigma>) = distributed M lborel (\<lambda>x. (X x - \<mu>) / \<sigma>) standard_normal_density"
+proof auto
   assume "distributed M lborel X (\<lambda>x. ereal (normal_density \<mu> \<sigma> x))"
   then have "distributed M lborel (\<lambda>x. -\<mu> / \<sigma> + (1/\<sigma>) * X x) (\<lambda>x. ereal (normal_density (-\<mu> / \<sigma> + (1/\<sigma>)* \<mu>) (\<bar>1/\<sigma>\<bar> * \<sigma>) x))"
     by(rule normal_density_affine) auto
   
   then show "distributed M lborel (\<lambda>x. (X x - \<mu>) / \<sigma>) (\<lambda>x. ereal (standard_normal_density x))"
-    by (simp add: uminus_add_conv_diff diff_divide_distrib[symmetric] field_simps)
+    by (simp add: diff_divide_distrib[symmetric] field_simps)
 next
   assume *: "distributed M lborel (\<lambda>x. (X x - \<mu>) / \<sigma>) (\<lambda>x. ereal (standard_normal_density x))"
   have "distributed M lborel (\<lambda>x. \<mu> + \<sigma> * ((X x - \<mu>) / \<sigma>)) (\<lambda>x. ereal (normal_density \<mu> \<bar>\<sigma>\<bar> x))"
@@ -272,7 +332,10 @@ proof -
   then have [simp]:"distributed M lborel (\<lambda>x. - Y x) (\<lambda>x. ereal (normal_density (- \<nu>) \<tau> x))" by simp
 
   have "distributed M lborel (\<lambda>x. X x + (- Y x)) (normal_density (\<mu> + - \<nu>) (sqrt (\<sigma>\<^sup>2 + \<tau>\<^sup>2)))"
-    by (intro sum_indep_normal indep_var_neg) simp_all
+    apply (rule sum_indep_normal)
+    apply (rule indep_var_compose[unfolded comp_def, of borel _ borel _ "\<lambda>x. x" _ "\<lambda>x. - x"])
+    apply simp_all
+    done
   then show ?thesis by simp
 qed
 
@@ -288,12 +351,13 @@ next
   case (insert i I)
     then have 1: "distributed M lborel (\<lambda>x. (X i x) + (\<Sum>i\<in>I. X i x)) 
                 (normal_density (\<mu> i  + setsum \<mu> I)  (sqrt ((\<sigma> i)\<^sup>2 + (sqrt (\<Sum>i\<in>I. (\<sigma> i)\<^sup>2))\<^sup>2)))"
-      by (intro sum_indep_normal indep_vars_setsum insert real_sqrt_gt_zero setsum_pos_pos)  
-         (auto intro: indep_vars_subset, fastforce)
-         
+      apply (intro sum_indep_normal indep_vars_setsum insert real_sqrt_gt_zero)  
+      apply (auto intro: indep_vars_subset intro!: setsum_pos)
+      apply fastforce
+      done
     have 2: "(\<lambda>x. (X i x)+ (\<Sum>i\<in>I. X i x)) = (\<lambda>x. (\<Sum>j\<in>insert i I. X j x))"
           "\<mu> i + setsum \<mu> I = setsum \<mu> (insert i I)"
-      using insert by (auto simp: random_vars_insert)    
+      using insert by auto
   
     have 3: "(sqrt ((\<sigma> i)\<^sup>2 + (sqrt (\<Sum>i\<in>I. (\<sigma> i)\<^sup>2))\<^sup>2)) = (sqrt (\<Sum>i\<in>insert i I. (\<sigma> i)\<^sup>2))"
       using insert by (simp add: setsum_nonneg)
@@ -308,19 +372,20 @@ proof -
 
   have 1: "(\<integral>\<^sup>+x. ereal (x * exp (- x\<^sup>2)) * indicator {0..} x \<partial>lborel) =ereal( 0 - ?F 0)"
   apply (rule nn_integral_FTC_atLeast)
-  apply (auto intro!: derivative_eq_intros simp: mult_nonneg_nonneg)
-  apply (rule tendsto_minus_cancel, simp add: field_simps)
+  apply (auto intro!: derivative_eq_intros)
+  apply (rule tendsto_minus_cancel)
+  apply (simp add: field_simps)
   proof - 
     have "((\<lambda>(x::real). exp (- x\<^sup>2) / 2) ---> 0 / 2) at_top"
     apply (intro tendsto_divide filterlim_compose[OF exp_at_bot] filterlim_compose[OF filterlim_uminus_at_bot_at_top])
-    by auto
+    apply auto
+    done
     then show "((\<lambda>(x::real). exp (- x\<^sup>2) / 2) ---> 0) at_top" by simp
   qed
 
   also have 2: "(\<integral>\<^sup>+x. ereal (x * exp (- x\<^sup>2)) * indicator {0..} x \<partial>lborel) = integral\<^sup>N lborel (\<lambda>x. ereal (x * exp (- x\<^sup>2)))"
-    apply (subst(2) nn_integral_max_0[symmetric])
-    unfolding max_def 
-    by (auto intro!: nn_integral_cong split:split_indicator simp: mult_nonneg_nonneg zero_le_mult_iff)
+    by (subst(2) nn_integral_max_0[symmetric])
+       (auto intro!: nn_integral_cong split: split_indicator simp: max_def zero_le_mult_iff)
   finally show "(\<integral>\<^sup>+x. ereal (x * exp (- x\<^sup>2)) \<partial>lborel) = ereal 1 / 2" by auto
 
   show "(\<integral>\<^sup>+x. ereal (x * exp (- x\<^sup>2)) * indicator {0..} x \<partial>lborel) = ereal 1 / 2" using 1 by auto
@@ -332,41 +397,42 @@ lemma borel_integral_x_times_standard_normal[intro]: "(\<integral>x. standard_no
   and borel_integrable_x_times_standard_normal'[intro]: "integrable lborel (\<lambda>x. x * standard_normal_density x)"
 proof -    
   have 0: "(\<integral>\<^sup>+x. ereal (x * standard_normal_density x) \<partial>lborel) = \<integral>\<^sup>+x. ereal (x * standard_normal_density x) * indicator {0..} x \<partial>lborel"
-    apply(subst nn_integral_max_0[symmetric]) 
+    apply (subst nn_integral_max_0[symmetric]) 
     unfolding max_def standard_normal_density_def
-    apply(auto intro!: nn_integral_cong split:split_indicator 
-      simp: mult_nonneg_nonneg divide_nonneg_nonneg zero_le_divide_iff zero_le_mult_iff)
-    by (metis not_le pi_gt_zero)
+    apply (auto intro!: nn_integral_cong split:split_indicator simp: zero_le_divide_iff zero_le_mult_iff)
+    apply (metis not_le pi_gt_zero)
+    done
 
   have 1: "(\<integral>\<^sup>+x. ereal (- (x * standard_normal_density x)) \<partial>lborel) = \<integral>\<^sup>+x. ereal (x * standard_normal_density x) * indicator {0..} x \<partial>lborel"
     apply (subst(2) nn_integral_real_affine[where c = "-1" and t = 0])
-    apply(auto simp: standard_normal_density_def split:split_indicator simp: mult_nonneg_nonneg divide_nonneg_nonneg)
+    apply(auto simp: standard_normal_density_def split: split_indicator)
     apply(subst nn_integral_max_0[symmetric]) 
     unfolding max_def standard_normal_density_def
-    by(auto intro!: nn_integral_cong split:split_indicator 
-      simp: mult_nonneg_nonneg divide_nonneg_nonneg divide_le_0_iff mult_le_0_iff)
-     (metis not_le pi_gt_zero)
-  
+    apply (auto intro!: nn_integral_cong split: split_indicator
+                simp: divide_le_0_iff mult_le_0_iff one_ereal_def[symmetric])
+    apply (metis not_le pi_gt_zero)
+    done
+
   have 2: "sqrt pi / sqrt 2 * (\<integral>\<^sup>+x. ereal (x * standard_normal_density x) * indicator {0..} x \<partial>lborel) = integral\<^sup>N lborel (\<lambda>x. ereal (x * exp (- x\<^sup>2)))"
     unfolding standard_normal_density_def
     apply (subst nn_integral_real_affine[where c = "sqrt 2" and t = 0])
-    apply (auto simp: mult_nonneg_nonneg divide_nonneg_nonneg power_mult_distrib split: split_indicator)
+    apply (auto simp: power_mult_distrib split: split_indicator)
     apply (subst mult_assoc[symmetric])
     apply (subst nn_integral_cmult[symmetric])
-    apply (auto simp: mult_nonneg_nonneg)
+    apply auto
     apply (subst(2) nn_integral_max_0[symmetric])
-    unfolding max_def 
-    by (auto intro!: nn_integral_cong split:split_indicator simp:mult_nonneg_nonneg zero_le_mult_iff real_sqrt_mult)
+    apply (auto intro!: nn_integral_cong split: split_indicator simp: max_def zero_le_mult_iff real_sqrt_mult)
+    done
 
   have *: "(\<integral>\<^sup>+x. ereal (x * standard_normal_density x) * indicator {0..} x \<partial>lborel) = sqrt 2 / sqrt pi *(integral\<^sup>N lborel (\<lambda>x. ereal (x * exp (- x\<^sup>2))))"
     apply (subst 2[symmetric])
     apply (subst mult_assoc[symmetric])
-    by (auto simp: field_simps)
+    apply (auto simp: field_simps one_ereal_def[symmetric])
+    done
     
   show "(\<integral> x. x * standard_normal_density x \<partial>lborel) = 0" "integrable lborel (\<lambda>x. x * standard_normal_density x)"
-    apply (subst real_lebesgue_integral_def)
-    unfolding real_integrable_def
-    by (auto simp: 0 1 * nn_integral_x_exp_x_square)
+    by (subst real_lebesgue_integral_def)
+       (auto simp: 0 1 * nn_integral_x_exp_x_square real_integrable_def)
 
   then show "(\<integral> x. standard_normal_density x * x \<partial>lborel) = 0" "integrable lborel (\<lambda>x. standard_normal_density x * x)"
     by (simp_all add:mult_commute)
@@ -382,39 +448,39 @@ lemma (in prob_space) normal_distributed_expectation:
   assumes D: "distributed M lborel X (normal_density \<mu> \<sigma>)"
   shows "expectation X = \<mu>"
 proof -
-  have D1: "distributed M lborel (\<lambda>x. (X x - \<mu>) / \<sigma>) standard_normal_density"
+  def X' \<equiv> "\<lambda>x. (X x - \<mu>) / \<sigma>"
+  then have D1: "distributed M lborel X' standard_normal_density"
     by (simp add: normal_standard_normal_convert[OF pos_var, of X \<mu>, symmetric] D)
+  then have [simp]: "integrable M X'"
+    by (rule distributed_integrable_var) auto
 
-  have "expectation X = expectation (\<lambda>x. \<mu> + \<sigma> * (\<lambda>x. (X x - \<mu>) / \<sigma>) x)" by simp
-  also have "... = \<mu> + \<sigma>*(expectation (\<lambda>x. (X x - \<mu>) / \<sigma>))"
-    by(subst expectation_affine[OF D1]) (auto simp: prob_space_normal_density)    
-  also have "... = \<mu>"
-    by (auto simp: standard_normal_distributed_expectation[OF D1] simp del: integral_divide_zero)
-  finally show ?thesis .
+  have "expectation X = expectation (\<lambda>x. \<mu> + \<sigma> * X' x)"
+    by (simp add: X'_def)
+  then show ?thesis
+    by (simp add: prob_space standard_normal_distributed_expectation[OF D1])
 qed
 
 lemma integral_xsquare_exp_xsquare: "(\<integral> x. (x\<^sup>2 * exp (-x\<^sup>2 )) \<partial>lborel) =  sqrt pi / 2"
   and integrable_xsquare_exp_xsquare: "integrable lborel (\<lambda>x. x\<^sup>2 * exp (- x\<^sup>2)::real)"
 proof- 
-  note mult_nonneg_nonneg[simp]
   note filterlim_compose[OF exp_at_top, intro] filterlim_ident[intro]
 
   let ?f = "(\<lambda>x. x * - exp (- x\<^sup>2) / 2 - 0 * - exp (- 0\<^sup>2) / 2 -
                  \<integral> xa. 1 * (- exp (- xa\<^sup>2) / 2) * indicator {0..x} xa \<partial>lborel)::real\<Rightarrow>real"
   let ?IFunc = "(\<lambda>z. \<integral>x. (x\<^sup>2 * exp (- x\<^sup>2)) * indicator {0 .. z} x \<partial>lborel)::real\<Rightarrow>real"
 
-  have 1: "(\<integral>\<^sup>+xa. ereal (exp (- xa\<^sup>2)) * indicator {0..} xa \<partial>lborel) = ereal (sqrt pi) / ereal 2"
-    apply (subst nn_integral_ereal_indicator_mult)
-    apply (subst gaussian_integral_positive[symmetric])
-    apply (subst(2) nn_integral_even_function) 
-    apply (auto simp: field_simps)
-    by (cases "\<integral>\<^sup>+x. ereal (indicator {0..} x * exp (- x\<^sup>2)) \<partial>lborel") auto
 
-  have I: "(\<integral>xa. exp (- xa\<^sup>2) * indicator {0..} xa \<partial>lborel) = sqrt pi / 2"
-    apply (rule lebesgue_integral_eq_nn_integral)
-    apply (subst nn_integral_ereal_indicator_mult[symmetric])
-    apply (subst 1)
-    by (auto split:split_indicator)
+  from nn_integral_gaussian  
+  have 1: "(\<integral>\<^sup>+xa. ereal (exp (- xa\<^sup>2)) * indicator {0..} xa \<partial>lborel) = ereal (sqrt pi) / ereal 2"
+    apply (subst (asm) nn_integral_even_function)
+    apply simp
+    apply simp
+    apply (cases "\<integral>\<^sup>+ xa. ereal (exp (- xa\<^sup>2)) * indicator {0..} xa \<partial>lborel")
+    apply auto
+    done
+
+  then have I: "(\<integral>xa. exp (- xa\<^sup>2) * indicator {0..} xa \<partial>lborel) = sqrt pi / 2"
+    by (subst integral_eq_nn_integral) (auto simp: ereal_mult_indicator)
   
   have byparts: "?IFunc = (\<lambda>z. (if z < 0 then 0 else ?f z))"
     proof (intro HOL.ext, subst split_ifs, safe)
@@ -449,18 +515,24 @@ proof-
     then show ?thesis by simp
   qed
 
-  have [intro]: "((\<lambda>x. \<integral>y. exp (- y\<^sup>2) * indicator {0..x} y \<partial>lborel :: real) ---> \<integral>y. exp (- y\<^sup>2) * indicator {0..} y \<partial>lborel) at_top"
-    by(auto intro!: tendsto_mult_indicator)
+  have "((\<lambda>x. (\<integral>y. (exp (- y\<^sup>2) * indicator {0..} y) * indicator {.. x} y \<partial>lborel) :: real) ---> \<integral>y. exp (- y\<^sup>2) * indicator {0..} y \<partial>lborel) at_top"
+    by (intro tendsto_integral_at_top integrable_mult_indicator) auto
+  also have "(\<lambda>x. (\<integral>y. (exp (- y\<^sup>2) * indicator {0..} y) * indicator {.. x} y \<partial>lborel) :: real) = 
+    (\<lambda>x. (\<integral>y. exp (- y\<^sup>2) * indicator {0..x} y \<partial>lborel) :: real)"
+    by (auto simp: fun_eq_iff split: split_indicator intro!: integral_cong)
+  finally have *: "((\<lambda>x. (\<integral>y. exp (- y\<^sup>2) * indicator {0..x} y \<partial>lborel) :: real) ---> \<integral>y. exp (- y\<^sup>2) * indicator {0..} y \<partial>lborel) at_top"
+    .
 
   have tends: "((\<lambda>x. (\<integral> xa. exp (- xa\<^sup>2) * indicator {0..x} xa \<partial>lborel) / 2) ---> (sqrt pi / 2) / 2) at_top"
     apply (rule tendsto_divide)
-    by (subst I[symmetric]) auto
+    apply (subst I[symmetric])
+    apply (auto intro: *)
+    done
 
   have [intro]: "(?IFunc ---> sqrt pi / 4) at_top"
     apply (simp add: byparts)
     apply (subst filterlim_cong[where g = ?f])
-    apply (auto simp: eventually_ge_at_top linorder_not_less
-      divide_minus_left)
+    apply (auto simp: eventually_ge_at_top linorder_not_less)
   proof -
     have "((\<lambda>x. (\<integral> xa. exp (- xa\<^sup>2) * indicator {0..x} xa / 2 \<partial>lborel) - x * exp (- x\<^sup>2) / 2::real) --->
         (0 + sqrt pi / 4 - 0)) at_top"
@@ -485,11 +557,15 @@ proof-
   then have "(\<integral>\<^sup>+x. ereal (x\<^sup>2 * exp (- x\<^sup>2)* indicator {0..} x) \<partial>lborel) = sqrt pi / 4"
     by (subst nn_integral_eq_integral) auto
 
-  then have ***: "(\<integral>\<^sup>+ x.  ereal (x\<^sup>2 * exp (- x\<^sup>2)) \<partial>lborel) = sqrt pi / 2"
-    by (auto simp: real_sqrt_mult real_sqrt_divide nn_integral_even_function)
+  then have ***: "(\<integral>\<^sup>+ x. ereal (x\<^sup>2 * exp (- x\<^sup>2)) \<partial>lborel) = sqrt pi / 2"
+    by (subst nn_integral_even_function)
+       (auto simp: real_sqrt_mult real_sqrt_divide ereal_mult_indicator)
   
-  show "(\<integral> x. x\<^sup>2 * exp (- x\<^sup>2) \<partial>lborel) = sqrt pi / 2" "integrable lborel (\<lambda>x. x\<^sup>2 * exp (- x\<^sup>2)::real)"
-    by (auto simp: lebesgue_integral_eq_nn_integral[OF ***] integrable_if_nn_integral[OF ***])
+  then show "(\<integral> x. x\<^sup>2 * exp (- x\<^sup>2) \<partial>lborel) = sqrt pi / 2"
+    by (subst integral_eq_nn_integral) auto
+
+  show "integrable lborel (\<lambda>x. x\<^sup>2 * exp (- x\<^sup>2)::real)"
+    by (intro integrableI_nn_integral_finite[OF _ _ ***]) auto
 qed
 
 lemma integral_xsquare_times_standard_normal[intro]: "(\<integral> x. standard_normal_density x * x\<^sup>2 \<partial>lborel) = 1"
@@ -513,7 +589,7 @@ proof -
 
   show "integrable lborel (\<lambda>x. standard_normal_density x * x\<^sup>2)"
     unfolding standard_normal_density_def
-    apply (subst integrable_affine[where c = "sqrt 2" and t=0])
+    apply (subst lborel_integrable_real_affine_iff[where c = "sqrt 2" and t=0, symmetric])
     by (auto simp: power_mult_distrib real_sqrt_mult)
 qed
 
@@ -539,7 +615,8 @@ proof -
  
   show "integrable lborel (\<lambda>x. normal_density \<mu> \<sigma> x * (x - \<mu>)\<^sup>2)"
     unfolding normal_density_def
-    apply (subst integrable_affine[ where c = \<sigma> and t = \<mu>], auto)
+    apply (subst lborel_integrable_real_affine_iff[ where c = \<sigma> and t = \<mu>, symmetric])
+    apply auto
     apply (auto simp: power_mult_distrib)
     apply (subst integrable_cong[where g ="(\<lambda>x. \<sigma> * (standard_normal_density x * x\<^sup>2))"], auto)
     unfolding standard_normal_density_def
@@ -577,39 +654,22 @@ qed
 lemma (in information_space) entropy_normal_density:
   assumes [arith]: "0 < \<sigma>"
   assumes D: "distributed M lborel X (normal_density \<mu> \<sigma>)"
-  shows "entropy b lborel X =  log b (2 * pi * exp 1 * \<sigma>\<^sup>2) / 2"
-proof (subst entropy_distr[OF D])
-  (* have to use lebesgue integral here, wanted to use positive integral but this function is 
-     ot positive for all x > 0 *)
-  (* can not convert to standard normal density as it resutls in goal
-     @{term "integrable lborel (\<lambda>x. standard_normal_density x * log b _)"}, or something of this
-     form after applying integral_cmult after lebesgue_integral_real_affine *)
-  let ?I = "- (\<integral> x. normal_density \<mu> \<sigma> x * log b (normal_density \<mu> \<sigma> x) \<partial>lborel)"
-  note integrable_xsquare_times_normal[OF assms(1), intro] 
-       integrable_normal[OF assms(1), intro]
-       times_divide_eq_left[simp del]
-
-  have 1: "\<And>x. log b (normal_density \<mu> \<sigma> x) = (- ln (2 * pi * \<sigma>\<^sup>2) - (x - \<mu>)\<^sup>2 / \<sigma>\<^sup>2) / (2 * ln b)"
-    unfolding normal_density_def
-    by(auto simp: ln_mult add_divide_distrib diff_divide_distrib log_def ln_div ln_sqrt)    
-
-  have "?I = (ln (sqrt (2 * pi * \<sigma>\<^sup>2)) / ln b ) * (\<integral> x. normal_density \<mu> \<sigma> x \<partial>lborel)
-       + (1 / (\<sigma>\<^sup>2 * (2 * ln b))) * \<integral> x. normal_density \<mu> \<sigma> x * (x - \<mu>)\<^sup>2 \<partial>lborel"
-    unfolding integral_minus[symmetric] integral_mult_left_zero[symmetric] integral_mult_right_zero[symmetric]
-    apply (subst integral_add[symmetric])
-    apply (auto simp: 1) []
-    apply (auto simp: 1) []
-    apply (intro integral_cong)
-    apply (auto simp: 1 field_simps ln_sqrt minus_divide_left add_divide_distrib)
-    done
-
-  also have "... = log b (2 * pi * exp 1 * \<sigma>\<^sup>2) / 2"
-    apply (subst integral_xsquare_times_normal[OF assms(1)])
-    apply (subst integral_normal_density)
-    apply (auto simp: field_simps log_def ln_sqrt ln_mult)
-    by (auto simp: add_divide_distrib)
-
-  finally show "?I = log b (2 * pi * exp 1 * \<sigma>\<^sup>2) / 2" .
+  shows "entropy b lborel X = log b (2 * pi * exp 1 * \<sigma>\<^sup>2) / 2"
+proof -
+  have "entropy b lborel X = - (\<integral> x. normal_density \<mu> \<sigma> x * log b (normal_density \<mu> \<sigma> x) \<partial>lborel)"
+    using D by (rule entropy_distr)
+  also have "\<dots> = - (\<integral> x. normal_density \<mu> \<sigma> x * (- ln (2 * pi * \<sigma>\<^sup>2) - (x - \<mu>)\<^sup>2 / \<sigma>\<^sup>2) / (2 * ln b) \<partial>lborel)"
+    by (intro arg_cong[where f="uminus"] integral_cong)
+       (auto simp: normal_density_def field_simps ln_mult log_def ln_div ln_sqrt)
+  also have "\<dots> = - (\<integral>x. - (normal_density \<mu> \<sigma> x * (ln (2 * pi * \<sigma>\<^sup>2)) + (normal_density \<mu> \<sigma> x * (x - \<mu>)\<^sup>2) / \<sigma>\<^sup>2) / (2 * ln b) \<partial>lborel)"
+    by (intro arg_cong[where f="uminus"] integral_cong) (auto simp: divide_simps field_simps)
+  also have "\<dots> = (\<integral>x. normal_density \<mu> \<sigma> x * (ln (2 * pi * \<sigma>\<^sup>2)) + (normal_density \<mu> \<sigma> x * (x - \<mu>)\<^sup>2) / \<sigma>\<^sup>2 \<partial>lborel) / (2 * ln b)"
+    by (simp del: minus_add_distrib)
+  also have "\<dots> = (ln (2 * pi * \<sigma>\<^sup>2) + 1) / (2 * ln b)"
+    by (simp add: integrable_xsquare_times_normal integrable_normal integral_xsquare_times_normal)
+  also have "\<dots> = log b (2 * pi * exp 1 * \<sigma>\<^sup>2) / 2"
+    by (simp add: log_def field_simps ln_mult)
+  finally show ?thesis .
 qed
 
 end
