Analysis/Characteristic_Functions.thy
@@ -5,7 +5,7 @@ Authors: Jeremy Avigad, Luke Serafin
 
 theory Characteristic_Functions
 
-imports Weak_Convergence Real_to_Complex Independent_Family Si Auxiliary Normal_Moments
+imports Weak_Convergence Real_to_Complex Independent_Family Si Normal_Moments
 
 begin
 
